Add C toy lang to proofmode

theories/language/lifting.v
@@ -6,7 +6,7 @@ From melocoton.language Require Export weakestpre.
 From iris.prelude Require Import options.
 
 Section lifting.
-Context `{!irisGS_gen hlc val pubstate Λ Σ}.
+Context `{!melocotonGS_gen hlc val pubstate Λ Σ}.
 Implicit Types prog : mixin_prog (func Λ).
 Implicit Types s : prog_environ.
 Implicit Types v : val.
@@ -38,7 +38,7 @@ Lemma wp_lift_atomic_step {s E Φ} e1 :
   to_val e1 = None →
   (∀ σ1 ns, state_interp σ1 ns ={E}=∗
     ⌜reducible (prog s) e1 σ1⌝ ∗
-    ▷ ∀ e2 σ2, ⌜prim_step (prog s) e1 σ1 e2 σ2 []⌝ -∗
+    ▷ ∀ e2 σ2, ⌜prim_step (prog s) e1 σ1 e2 σ2 []⌝ ={E}=∗
       state_interp σ2 (S ns) ∗
       from_option Φ False (to_val e2))
   ⊢ WP e1 @ s; E {{ Φ }}.
@@ -46,8 +46,29 @@ Proof.
   iIntros (?) "H".
   iApply (wp_lift_step_fupd s E _ e1)=>//; iIntros (σ1 ns) "Hσ1".
   iMod ("H" $! σ1 with "Hσ1") as "[$ H]". iModIntro.
-  iIntros (e' σ' Hstep). do 4 iModIntro.
-  iDestruct ("H" $! e' σ' Hstep) as "[H1 H2]".
+  iIntros (e' σ' Hstep). do 3 iModIntro.
+  iMod ("H" $! e' σ' Hstep) as "[H1 H2]". iModIntro.
+  iFrame.
+  destruct (to_val e') eqn:?; last by iExFalso.
+  iApply wp_value; first done. iApply "H2".
+Qed.
+
+
+
+Lemma wp_lift_atomic_head_step {s E Φ} e1 :
+  to_val e1 = None →
+  (∀ σ1 ns, state_interp σ1 ns ={E}=∗
+    ⌜head_reducible (prog s) e1 σ1⌝ ∗
+    ▷ ∀ e2 σ2, ⌜head_step (prog s) e1 σ1 e2 σ2 []⌝ ={E}=∗
+      state_interp σ2 (S ns) ∗
+      from_option Φ False (to_val e2))
+  ⊢ WP e1 @ s; E {{ Φ }}.
+Proof.
+  iIntros (?) "H".
+  iApply (wp_lift_step_fupd s E _ e1)=>//; iIntros (σ1 ns) "Hσ1".
+  iMod ("H" $! σ1 with "Hσ1") as "[%HH H]". iModIntro. iSplitR; first (iPureIntro; by eapply head_prim_reducible).
+  iIntros (e' σ' Hstep%head_reducible_prim_step). 2:easy. do 3 iModIntro.
+  iMod ("H" $! e' σ' Hstep) as "[H1 H2]". iModIntro.
   iFrame.
   destruct (to_val e') eqn:?; last by iExFalso.
   iApply wp_value; first done. iApply "H2".
@@ -75,9 +96,33 @@ Qed.
       prim_step p e1 σ1 e2' σ2 efs → σ2 = σ1 ∧ e2' = e2 ∧ efs = []
   }.
 
+  Record pure_head_step (p : language.prog Λ) (e1 e2 : expr Λ) := {
+    pure_head_step_safe σ1 : head_reducible p e1 σ1;
+    pure_head_step_det σ1 e2' σ2 efs :
+      head_step p e1 σ1 e2' σ2 efs → σ2 = σ1 ∧ e2' = e2 ∧ efs = []
+  }.
+
+  Lemma pure_head_step_pure_step p e1 e2 : pure_head_step p e1 e2 -> pure_step p e1 e2.
+  Proof.
+    intros [Hp1 Hp2]. split.
+    - intros σ. destruct (Hp1 σ) as (e2' & σ2 & efs & ?).
+      eexists e2', σ2, efs. by apply head_prim_step.
+    - intros σ1 e2' σ2 efs ?%head_reducible_prim_step; eauto.
+  Qed.
+
 Class PureExec (φ : Prop) (n : nat)  (p : language.prog Λ) (e1 e2 : expr Λ) :=
   pure_exec : φ → relations.nsteps (pure_step p) n e1 e2.
 
+Lemma pure_exec_fill φ n p e1 e2 K : PureExec φ n p  e1 e2 -> PureExec φ n p (fill K e1) (fill K e2).
+Proof.
+  intros H Hφ. specialize (H Hφ). induction H as [|n x y z [Hred Hdet] Hstep IH]; econstructor.
+  - econstructor.
+    + intros σ1. destruct (Hred σ1) as (e' & σ' & efs' & H). do 3 eexists.
+      apply fill_prim_step, H.
+    + intros σ1 e2 σ2 efs (e2' & -> & HH)%fill_reducible_prim_step; last apply Hred.
+      destruct (Hdet _ _ _ _ HH) as (-> & -> & ->); done.
+  - apply IH.
+Qed.
 
 Lemma wp_pure_step_fupd `{!Inhabited (state Λ)} s E e1 e2 φ n Φ :
   PureExec φ n (prog s) e1 e2 →
