theories/c_toy_lang/iris/adequacy.v
@@ -2,7 +2,7 @@ From iris.algebra Require Import auth.
 From iris.base_logic.lib Require Import mono_nat.
 From iris.proofmode Require Import proofmode.
 From iris.program_logic Require Export weakestpre adequacy.
-From melocoton.c_toy_lang Require Import proofmode notation.
+From melocoton.c_toy_lang Require Import iris.proofmode notation.
 From iris.prelude Require Import options.
 
 Class heapGpreS Σ := HeapGpreS {
