theories/c_toy_lang/melocoton/class_instances.v
@@ -1,0 +1,76 @@
+From melocoton.language Require Export weakestpre lifting.
+From melocoton.c_toy_lang Require Export lang.
+From melocoton.c_toy_lang Require Import tactics melocoton.tactics notation.
+From iris.prelude Require Import options.
+
+Section pure_exec.
+  Context {p:program}.
+  Local Ltac solve_exec_safe := intros; subst; do 3 eexists; try (repeat (econstructor; eauto); done).
+  Local Ltac solve_exec_puredet := simpl; intros; inv_head_step; try done.
+  Local Ltac solve_pure_exec :=
+    subst; intros ?; apply nsteps_once, pure_head_step_pure_step;
+      constructor; [solve_exec_safe | solve_exec_puredet].
+
+  Local Ltac destruct_bool_decide := repeat (let H := fresh "Heq" in 
+    try destruct bool_decide eqn:H; 
+    [apply bool_decide_eq_true_1 in H| apply bool_decide_eq_false_1 in H]).
+
+  Global Instance pure_let x (v1 v2 : val) :
+    PureExec True 1 p (Let x (Val v1) (Val v2)) (subst' x v1 v2).
+  Proof. solve_pure_exec. Qed.
+
+  Global Instance pure_unop op v v' :
+    PureExec (un_op_eval op v = Some v') 1 p (UnOp op (Val v)) (Val v').
+  Proof. solve_pure_exec. Qed.
+
+  Global Instance pure_binop op v1 v2 v' :
+    PureExec (bin_op_eval op v1 v2 = Some v') 1 p (BinOp op (Val v1) (Val v2)) (Val (LitV v')) | 10.
+  Proof. solve_pure_exec. Qed.
+
+  (* Higher-priority instance for [EqOp]. *)
+  Global Instance pure_eqop v1 v2 :
+    PureExec (vals_compare_safe v1 v2) 1 p
+      (BinOp EqOp (Val (LitV v1)) (Val (LitV v2)))
+      (Val $ LitV $ LitBool $ bool_decide (v1 = v2)) | 1.
+  Proof.
+    intros Hcompare.
+    cut (bin_op_eval EqOp (LitV v1) (LitV v2) = Some $ LitBool $ bool_decide (v1 = v2)).
+    { intros. revert Hcompare. solve_pure_exec. }
+    destruct v1, v2; cbn in *; try easy.
+    - destruct_bool_decide; congruence.
+    - destruct l, l0. destruct_bool_decide; congruence.
+    - destruct_bool_decide; congruence.
+  Qed.
+
+  Global Instance pure_if_true v e1 e2 : asTruth v = true ->
+    PureExec True 1 p (If (Val $ v) e1 e2) e1.
+  Proof. intros H. solve_pure_exec. congruence. Qed.
+  Global Instance pure_if_non_zero (v0:Z) e1 e2 : v0 ≠ 0%Z ->
+    PureExec True 1 p (If (Val $ LitV $ LitInt v0) e1 e2) e1.
+  Proof. intros H. apply pure_if_true. destruct v0; cbn; congruence. Qed.
+  Global Instance pure_if_true_bool e1 e2 :
+    PureExec True 1 p (If (Val $ LitV $ LitBool true) e1 e2) e1.
+  Proof. apply pure_if_true. easy. Qed.
+  Global Instance pure_if_false v e1 e2 : asTruth v = false ->
+    PureExec True 1 p (If (Val $ v) e1 e2) e2.
+  Proof. intros H. solve_pure_exec. congruence. Qed.
+  Global Instance pure_if_zero e1 e2 : 
+    PureExec True 1 p (If (Val $ LitV $ LitInt (0%Z)) e1 e2) e2.
+  Proof. apply pure_if_false. easy. Qed.
+  Global Instance pure_if_false_bool e1 e2 :
+    PureExec True 1 p (If (Val $ LitV $ LitBool false) e1 e2) e2.
+  Proof. apply pure_if_zero. Qed.
+
+  Global Instance pure_while e1 e2 : 
+    PureExec True 1 p (While e1 e2) (If e1 (Let BAnon e1 (While e1 e2)) (Val $ LitV $ LitInt 0)).
+  Proof. solve_pure_exec. Qed.
+
+  Global Instance pure_funcall s va args res e : 
+    PureExec ((p : gmap.gmap string function) !! s = Some (Fun args e) ∧ zip_args args va = Some res) 1 p (FunCall (Val $ LitV $ LitFunPtr s) (map Val va)) (subst_all res e).
+  Proof. solve_pure_exec; destruct H as [H1 H2].
+    1: do 2 econstructor. 1:apply H1.
+    + unfold apply_function. rewrite H2. reflexivity.
+    + repeat split; try congruence. destruct (zip_args args0 va) eqn:Heq; last congruence.
+      congruence.
+  Qed.
+End pure_exec.
